flush and compact left

Splinter/Betree/LikesBranchedBetree.i.dfy
@@ -1,7 +1,6 @@
 // Copyright 2018-2021 VMware, Inc., Microsoft Inc., Carnegie Mellon University, ETH Zurich, and University of Washington
 // SPDX-License-Identifier: BSD-2-Clause
 
-include "Branches.i.dfy"
 include "../Disk/GenericDisk.i.dfy"
 include "../Likes.i.dfy"
 include "Domain.i.dfy"
@@ -9,7 +8,6 @@ include "../../lib/Base/mathematics.i.dfy"
 include "../../lib/Base/Multisets.i.dfy"
 // include "../../lib/Buckets/BoundedPivotsLib.i.dfy"
 include "BranchedBetree.i.dfy"
-include "SplitRequest.i.dfy"
 
 module LikesBranchedBetreeMod
 {
@@ -28,28 +26,28 @@ module LikesBranchedBetreeMod
   // import opened ValueMessage
   import opened Maps
   // import TotalKMMapMod
-  // import opened SplitRequestMod
-  import opened BranchSeq
+  import opened SplitRequestMod
+  import opened BranchSeqMod
   import opened Multisets
   import opened LikesMod
 
   import M = Mathematics
   import BB = BranchedBetreeMod
+  import LB = LinkedBranchMod
 
   type Pointer = GenericDisk.Pointer
   type Address = GenericDisk.Address
   type Ranking = GenericDisk.Ranking
   type StampedBetree = Stamped<BB.BranchedBetree>
+  type BranchDiskView = LB.DiskView
 
-  // TODO: move to branch module
-  function BranchLikes(root: Address, branches: Branches) : Likes
+  function BranchLikes(root: Address, branchDiskView: BranchDiskView) : Likes
   {
-    NoLikes() 
+    var branch := LB.LinkedBranch(root, branchDiskView);
+    if branch.Acyclic() then multiset(branch.Representation()) else NoLikes()
   }
 
-
   function TransitiveLikes(bbtree: BB.BranchedBetree) : Likes
-    requires bbtree.WF()
     requires bbtree.Acyclic()
   {
     TransitiveLikesDefn(bbtree, bbtree.TheRanking())
@@ -69,9 +67,9 @@ module LikesBranchedBetreeMod
       NoLikes()
     else (
       var root := bbtree.Root();
-      var rootLikes := map[ root := 1 ];
-      var branchLikes := mapsum(map addr | addr in root.buffers :: BranchLikes(addr, bbtree.branches)); 
-      var childrenLikes := mapsum(map i | 0 <= i < |root.children| :: TransitiveLikes(bbtree.ChildAtIdx(i), r));
+      var rootLikes := multiset{bbtree.root.value};
+      var branchLikes := mapsum(map addr | addr in root.branches.Representation() :: BranchLikes(addr, bbtree.branchDiskView)); 
+      var childrenLikes := mapsum(map i | 0 <= i < |root.children| :: TransitiveLikesDefn(bbtree.ChildAtIdx(i), r));
       rootLikes + branchLikes + childrenLikes
     )
   }
@@ -79,7 +77,7 @@ module LikesBranchedBetreeMod
   function ImperativeLikes(v: Variables) : Likes
   {
     var branchLikes := mapsum(map addr | addr in v.branchLikes :: 
-      Multiply(BranchLikes(addr, v.branchedVars.branched.branches), v.branchLikes[addr]));
+      Multiply(BranchLikes(addr, v.branchedVars.branched.branchDiskView), v.branchLikes[addr]));
     branchLikes + v.betreeLikes
   }
 
@@ -87,8 +85,7 @@ module LikesBranchedBetreeMod
   predicate ImperativeAgreement(v: Variables) 
   {
     && v.branchedVars.branched.Acyclic()
-    // && v.branchedVars.branched.Valid()
-    && TransitiveLikes(v.branchedVars.branched, v.branchedVars.branched.TheRanking()) == ImperativeLikes(v)
+    && TransitiveLikes(v.branchedVars.branched) == ImperativeLikes(v)
   }
 
   datatype Variables = Variables(
@@ -96,8 +93,11 @@ module LikesBranchedBetreeMod
     branchedVars: BB.Variables,
   
     // plus imperatively-maintained view of the functional TransitiveLikes:
-    betreeLikes: Likes, // internal refs
-    branchLikes: Likes // outgoing refs
+    // internal refs, track # of times each betree node is referenced by another node
+    // should be 1 for tree, can be more after clone makes it a DAG
+    betreeLikes: Likes, 
+    // outgoing refs, track # of times each b+tree root is referenced by a betree node
+    branchLikes: Likes
   )
   {
     predicate WF() {
@@ -121,44 +121,123 @@ module LikesBranchedBetreeMod
   predicate InternalGrow(v: Variables, v': Variables, lbl: TransitionLabel, step: Step)
   {
     && lbl.InternalAllocationsLabel?
-    && BB.Next(v.branchedVars, v'.branchedVars, lbl.I())
-    // && BB.InternalGrow(v.branchedVars, v'.branchedVars, lbl.I(), step.I())
+    && step.InternalGrowStep?
+    && BB.NextStep(v.branchedVars, v'.branchedVars, lbl.I(), step.I())
     && v' == v.(
-      branchedVars := v'.branchedVars,  // admit relational update above
-      betreeLikes := v.betreeLikes
+      branchedVars := v'.branchedVars, // admit relational update above
+      betreeLikes := v.betreeLikes + multiset{step.newRootAddr}
     )
   }
 
-  predicate InternalCompact(v: Variables, v': Variables, lbl: TransitionLabel, step: Step)
+  predicate InternalFlushMemtable(v: Variables, v': Variables, lbl: TransitionLabel, step: Step)
   {
     && lbl.InternalAllocationsLabel?
-    && BB.Next(v.branchedVars, v'.branchedVars, lbl.I())
-//     && LinkedBetreeMod.InternalCompact(v.betree, v'.betree, lbl.I(), step.I())
+    && step.InternalFlushMemtableStep?
+    && BB.NextStep(v.branchedVars, v'.branchedVars, lbl.I(), step.I())
+    && var oldRoot := if v.branchedVars.branched.HasRoot() then multiset{v.branchedVars.branched.root.value} else multiset{};
+    && v' == v.(
+      branchedVars := v'.branchedVars, // admit relational update above
+      betreeLikes := v.betreeLikes - oldRoot + multiset{step.newRootAddr},
+      branchLikes := v.branchLikes + multiset{step.branch.root}
+    )
+  }
 
-    // should be in step
-    // && var root := v.branchedVars.branched.Root() 
-    // && var unlikedBranchRoots := multiset{Set(root.buffers[compactStart..compactEnd])};
-    // && var unlikedBetreeNodes := step.path.AddrsOnPath();
+  predicate InternalSplit(v: Variables, v': Variables, lbl: TransitionLabel, step: Step)
+  {
+    && lbl.InternalAllocationsLabel?
+    && step.InternalSplitStep?
+    && BB.NextStep(v.branchedVars, v'.branchedVars, lbl.I(), step.I())
 
-    // && v' == v.(
-    //   branchedVars := v'.branchedVars,  // admit relational update above
-    //   betreeLikes := v.betreeLikes + step.treeAddrs - unlikedBetreeNodes,
-    //   branchLikes := v.branchLikes + multiset{step.compactedBranch.root} - unlikedBranchRoots,
-    // )
+    && var node := v.branchedVars.branched.Root();
+    && v' == v.(
+      branchedVars := v'.branchedVars, // admit relational update above
+      betreeLikes := 
+        v.betreeLikes - multiset{node.children[step.request.childIdx].value} - multiset{ v.branchedVars.branched.root.value}
+        + multiset{step.newAddrs.parent} + multiset{step.newAddrs.left} + multiset{step.newAddrs.right}
+      // branchLikes do not change as a result
+    )
+  }
+
+  predicate InternalFlush(v: Variables, v': Variables, lbl: TransitionLabel, step: Step)
+  {
+    && lbl.InternalAllocationsLabel?
+    && step.InternalFlushStep?
+    && BB.NextStep(v.branchedVars, v'.branchedVars, lbl.I(), step.I())
+
+    && var node := v.branchedVars.branched.Root();
+    && v' == v.(
+      branchedVars := v'.branchedVars // admit relational update above
+    )
+  }
+
+//   predicate InternalCompact(v: Variables, v': Variables, lbl: TransitionLabel, step: Step)
+//   {
+//     && lbl.InternalAllocationsLabel?
+//     && BB.Next(v.branchedVars, v'.branchedVars, lbl.I())
+// //     && LinkedBetreeMod.InternalCompact(v.betree, v'.betree, lbl.I(), step.I())
+
+//     // should be in step
+//     // && var root := v.branchedVars.branched.Root() 
+//     // && var unlikedBranchRoots := multiset{Set(root.buffers[compactStart..compactEnd])};
+//     // && var unlikedBetreeNodes := step.path.AddrsOnPath();
+
+//     // && v' == v.(
+//     //   branchedVars := v'.branchedVars,  // admit relational update above
+//     //   betreeLikes := v.betreeLikes + step.treeAddrs - unlikedBetreeNodes,
+//     //   branchLikes := v.branchLikes + multiset{step.compactedBranch.root} - unlikedBranchRoots,
+//     // )
+//   }
+
+  predicate NoOp(v: Variables, v': Variables, lbl: TransitionLabel, step: Step)
+  {
+    && BB.NextStep(v.branchedVars, v'.branchedVars, lbl.I(), step.I())
+    && v' == v
   }
 
   datatype Step =
-    | InternalGrow(newRootAddr: Address)
-    | InternalCompact()
-    | InternalLabel()   // Local No-op label
+      QueryStep(receipt: BB.QueryReceipt)
+    | PutStep()
+    | QueryEndLsnStep()
+    | FreezeAsStep()
+    | InternalGrowStep(newRootAddr: Address)
+    | InternalSplitStep(path: BB.Path, request: SplitRequest, newAddrs: BB.L.SplitAddrs, pathAddrs: BB.PathAddrs)
+    | InternalFlushMemtableStep(newRootAddr: Address, branch: LB.LinkedBranch)
+    | InternalFlushStep(path: BB.Path, childIdx: nat, targetAddr: Address, targetChildAddr: Address, pathAddrs: BB.PathAddrs, branchGCCount: nat)
+    | InternalCompactStep(path: BB.Path, start: nat, end: nat, newBranch: LB.LinkedBranch, targetAddr: Address, pathAddrs: BB.PathAddrs)
+    | InternalNoOpStep()   // Local No-op label
   {
-  //   function I() : BB.TransitionLabel
-  //   {
-  //     match this {
-  //       case InternalAllocationsLabel(addrs) => BB.InternalAllocationsLabel(toSeq(addrs), [])
-  //       case _ => BB.InternalLabel
-  //     }
-  //   }
+    function I() : BB.Step
+    {
+      match this {
+        case QueryStep(receipt) => BB.QueryStep(receipt)
+        case PutStep() => BB.PutStep()
+        case QueryEndLsnStep() => BB.QueryEndLsnStep
+        case FreezeAsStep() => BB.FreezeAsStep()
+        case InternalGrowStep(newRootAddr) => BB.InternalGrowStep(newRootAddr)
+        case InternalFlushMemtableStep(newRootAddr, branch) => BB.InternalFlushMemtableStep(newRootAddr, branch)
+        case InternalFlushStep(path, childIdx, targetAddr, targetChildAddr, pathAddrs, branchGCCount) 
+          => BB.InternalFlushStep(path, childIdx, targetAddr, targetChildAddr, pathAddrs, branchGCCount)
+        case InternalCompactStep(path, start, end, newBranch, targetAddr, pathAddrs) 
+          => BB.InternalCompactStep(path, start, end, newBranch, targetAddr, pathAddrs) 
+        case _ => BB.InternalNoOpStep
+      }
+    }
   }
 
-} // module
+  predicate NextStep(v: Variables, v': Variables, lbl: TransitionLabel, step: Step)
+  {
+    match step {
+      case InternalGrowStep(_) => InternalGrow(v, v', lbl, step)
+      case InternalSplitStep(_, _, _, _) => InternalSplit(v, v', lbl, step)
+      case InternalFlushMemtableStep(_,_) => InternalFlushMemtable(v, v', lbl, step)
+      case InternalFlushStep(_, _, _, _, _, _) => InternalFlush(v, v', lbl, step)
+      // case InternalCompactStep(_, _, _, _, _, _) => InternalCompact(v, v', lbl, step)
+      case _ => NoOp(v, v', lbl, step)
+    }
+  }
+
+  predicate Next(v: Variables, v': Variables, lbl: TransitionLabel) {
+    exists step: Step :: NextStep(v, v', lbl, step)
+  }  
+
+} // moduleif v.betreeLikes[step] 
